progress on countableLib
Calling countableLib.count_datatype ty
on a recursive hol type ty with name "ty" defines
a new constant count_ty and
produces a pair of theorems
  |- INJ count_ty (UNIV:ty set) (UNIV:num set)
  |- countable (UNIV:ty set)
In case ty takes type arguments, it additionally defines another
constant count_ty_aux.

Still very much in-progress, because of the following missing features:
- Doesn't know about/remember other countable types, so will fail if
  ty has them in its leaves (almost every type is in this category!)
- Probably doesn't yet handle mutually recursive types
- Not sure what it does if ty is applied to non-variable type arguments

Tested on :α list, :num, and a few simple enumerations.

examples/miniML/computability/countableLib.sml
@@ -1,80 +1,82 @@
-open HolKernel pred_setTheory countableTheory lcsymtacs numSyntax pairSyntax
+open HolKernel pred_setTheory countableTheory lcsymtacs
+open boolSyntax numSyntax pairSyntax pred_setSyntax
 
-fun count_datatype ty = let
+val count_datatype = let
+  val count_num2 = ``count_num2``
+  fun mk_countable a = ``countable ^(mk_univ a)``
+  fun count_args ctr = let
+    fun f [] = term_of_int 0
+      | f [a] = mk_comb(ctr (type_of a), a)
+      | f (a::xs) = mk_comb(count_num2,mk_pair(mk_comb(ctr (type_of a), a),f xs))
+  in f end
+  fun mk_eqn ctr lhs0 (c,(n,eqs)) = let
+    val lhs = mk_comb(lhs0, c)
+    val (_,ars) = strip_comb c
+    val rhs = mk_comb(count_num2,mk_pair(term_of_int n,count_args ctr ars))
+    val eq = mk_eq (lhs, rhs)
+  in (n+1,eq::eqs) end
+  fun counter0 t = raise Fail "no memocache"
+in fn ty => let
   val axiom = TypeBase.axiom_of ty
   val (name,args) = dest_type ty
   val count_name = "count_"^name
-  val count_name_aux = count_name^"_aux"
-  val count_ty_tm = mk_var(count_name,ty --> num)
-  val helpers = map (fn a => genvar(a --> num)) args
-  val count_ty_aux_tm = mk_var(count_name_aux, foldl (fn (h,ty) => type_of h --> ty) (ty --> num) helpers)
-  val lhs0 = list_mk_comb (count_ty_aux_tm, helpers)
-  val constructors = TypeBase.constructors_of ty
-  fun args cty = let
-    val (d,r) = dom_rng cty
-  in genvar d :: args r end handle HOL_ERR _ => []
-  fun counter t = if t = ty then lhs0 else
-    Lib.first (fn h => fst(dom_rng(type_of h)) = t) helpers
-  val count_num2 = ``count_num2``
-  fun count_args [] = term_of_int 0
-    | count_args [a] = mk_comb(counter (type_of a), a)
-    | count_args (a::xs) = mk_comb(count_num2,mk_pair(mk_comb(counter (type_of a), a),count_args xs))
-  fun mk_eqn (c,(n,eqs)) = let
-    val ars = args (type_of c)
-    val lhs = mk_comb(lhs0, list_mk_comb (c,ars))
-    val rhs = mk_comb(count_num2,mk_pair(term_of_int n,count_args ars))
-    val eq = mk_eq (lhs, rhs)
-    in (n+1,eq::eqs) end
-  val (n,eqs) = foldl mk_eqn (0,[]) constructors
-  val count_ty_aux_def = new_recursive_definition
-                         {name=count_name_aux, rec_axiom=axiom,
-                          def=list_mk_conj eqs}
-in (count_ty_aux_def) end
+  val count_ty_var = mk_var(count_name,ty --> num)
+  val nchotomy = SPEC_ALL (TypeBase.nchotomy_of ty)
+  val constructors = map (rhs o snd o strip_exists) (strip_disj (concl nchotomy))
+in
+  if args = [] then let
+    val lhs0 = count_ty_var
+    fun counter t = if t = ty then lhs0 else counter0 t
+    val (_,eqs) = foldl (mk_eqn counter lhs0) (0,[]) constructors
+    val count_ty_def = new_recursive_definition
+                       {name=count_name, rec_axiom=axiom,
+                        def=list_mk_conj eqs}
+    val count_ty_tm = mk_const(count_name,ty --> num)
+    val count_ty_inj = prove(mk_inj(count_ty_tm,mk_univ ty,mk_univ num),
+      fs[INJ_DEF] >> Induct >> Cases >> fs[count_ty_def])
+    val countable_ty = prove(mk_countable ty,PROVE_TAC[count_ty_inj,countable_def])
+  in (count_ty_inj,countable_ty) end
+  else let
+    val helpers = map (fn a => genvar(a --> num)) args
+    val count_name_aux = count_name^"_aux"
+    val count_ty_aux_var = mk_var(count_name_aux,
+          foldl (fn (h,ty) => type_of h --> ty) (ty --> num) helpers)
+    val lhs0 = list_mk_comb (count_ty_aux_var, helpers)
+    fun counter t = if t = ty then lhs0 else
+      Lib.first (fn h => fst(dom_rng(type_of h)) = t) helpers
+      handle HOL_ERR _ => counter0 t
+    val (_,eqs) = foldl (mk_eqn counter lhs0) (0,[]) constructors
+    val count_ty_aux_def = new_recursive_definition
+                           {name=count_name_aux, rec_axiom=axiom,
+                            def=list_mk_conj eqs}
+    val count_ty_aux_tm = mk_const(count_name_aux, type_of count_ty_aux_var)
+    val count_ty_def = new_definition (count_name, mk_eq(count_ty_var,
+      mk_select(count_ty_var,mk_inj(count_ty_var,mk_univ ty,mk_univ num))))
+    val count_ty_tm = mk_const(count_name,ty --> num)
+    val hyps = map mk_countable args
+    val count_ty_inj = prove(
+      list_mk_imp(hyps,mk_inj(count_ty_tm,mk_univ ty,mk_univ num)),
+      simp_tac pure_ss [countable_def,count_ty_def] >>
+      foldl (fn (h,_) => disch_then (X_CHOOSE_THEN h assume_tac)) ALL_TAC helpers >>
+      SELECT_ELIM_TAC >> rw[] >>
+      exists_tac (list_mk_comb(count_ty_aux_tm,helpers)) >>
+      fs[INJ_DEF] >>
+      Induct >> rw[count_ty_aux_def] >>
+      qmatch_assum_rename_tac `X = (^count_ty_aux_tm Y) y` ["X","Y"] >>
+      Cases_on `y` >> fs[count_ty_aux_def])
+    val countable_ty = prove(list_mk_imp(hyps,mk_countable ty),
+                             PROVE_TAC[count_ty_inj,countable_def])
+  in (count_ty_inj,countable_ty) end
+end
+end
 
-val count_list_aux_def = count_datatype ``:α list``
-
-val list_countable = store_thm(
-"list_countable",
-``countable (UNIV:α set) ⇒ countable (UNIV:α list set)``,
-rw[countable_def] >>
-qexists_tac `count_list_aux f` >>
-fs[INJ_DEF] >>
-Induct >| [qx_gen_tac`y`,gen_tac >> qx_gen_tac`y`] >>
-rw[count_list_aux_def] >>
-ASSUME_TAC INJ_count_num2 >>
-Cases_on`y`>>fs[count_list_aux_def,INJ_DEF] >>
-res_tac >> fs[] >>
-res_tac >> fs[])
-
-val count_list_def = Define`
-  count_list = @f. INJ f (UNIV:α list set) (UNIV:num set)`
-
-val INJ_count_list = store_thm(
-"INJ_count_list",
-``countable (UNIV:α set) ⇒ INJ count_list (UNIV:α list set) UNIV``,
-rw[count_list_def] >>
-SELECT_ELIM_TAC >> rw[] >>
-metis_tac [list_countable,countable_def])
+val (count_list_inj, countable_list) = count_datatype ``:α list``
 
 open MiniMLTheory
-val count_error_aux_def = count_datatype ``:error``
+val (count_error_inj, countable_error) = count_datatype ``:error``
 
 (*
-val exp_countable = store_thm(
-"exp_countable",
-``countable (UNIV:exp set)``
-
-val count_v_def = Define`
-  (count_v (Lit l) = count_num2 (0, count_lit l))
-∧ (count_v (Conv cn vs) = count_num2 (1, count_num2(count_option cn, count_list count
-
-val v_countable = store_thm(
-"v_countable",
-``countable (UNIV:v set)``,
-rw[countable_def,INJ_DEF] >>
-qexists_tac `λv. case v of
-                 | Lit l => count_num2 (0,count_lit l)
-                 | Conv cn vs => count_num2 (1,count_num2(count_option cn, count_list vs))
-                 | Closure e n b => count_num2 (2,count_num2(count_list e,count_num2(count_string n,count_exp b)))
-                 | Recclosure
+val (count_lit_inj, countable_lit) = count_datatype ``:lit``
+val (count_result_inj, countable_result) = count_datatype ``:α result``
+val (count_exp_inj, countable_exp) = count_datatype ``:exp``
 *)
